Explored midstep-simulations

sepcomp/effect_semantics.v
@@ -360,6 +360,15 @@ Proof. intros; subst. eapply effstepN_trans; eassumption. Qed.
          eapply effstep_star_mem. apply EF.
   Qed.
 
+  Lemma corestepN_effstepN: forall n c1 m1 c2 m2, corestepN Sem g n c1 m1 c2 m2 ->
+       exists U, effstepN n U c1 m1 c2 m2.
+  Proof. induction n; simpl; intros.
+  + inv H. eexists; split; reflexivity.
+  + destruct H as [c [m [Step Steps]]].
+    apply effax2 in Step. destruct Step as [U1 HU1].
+    destruct (IHn _ _ _ _ Steps) as [U2 HU2]; clear IHn Steps.
+    do 5 eexists; split. eassumption. split. eassumption. reflexivity.
+  Qed.
 End effsemlemmas.
 
 
@@ -587,3 +596,739 @@ induction l; intros.
   - eapply free_curWR; eassumption.
 Qed.
 
+Inductive MidStepEffectResult {C:Type} :=
+  MSE_Ext: C -> mem -> (block -> Z -> bool) -> external_function -> list val -> MidStepEffectResult
+| MSE_Ret: C -> mem -> (block -> Z -> bool) -> val -> MidStepEffectResult
+| MSE_Div: (*(block -> Z -> bool) -> *)MidStepEffectResult. (*don't track written locations - ok for coarse grain, maybe not for instruction-level interleaving*)
+
+Inductive midstepE {G C} (SEM : @EffectSem G C) g (c:C) (m:mem):
+          @MidStepEffectResult C -> Prop:=
+  mse_ext: forall c' m' W f args,
+          effstep_star SEM g W c m c' m' ->
+          at_external SEM c' = Some (f,args) ->
+          midstepE SEM g c m (MSE_Ext c' m' W f args)
+| mse_ret: forall c' m' W v,
+          effstep_star SEM g W c m c' m' ->
+          halted SEM c' = Some v ->
+          midstepE SEM g c m (MSE_Ret c' m' W v)
+| mse_div: forall (H: forall n, exists c' m', corestepN SEM g n c m c' m'),
+          midstepE SEM g c m MSE_Div.
+(*using effstep_star implies that we're not tracking writes to newly allocated blocks - 
+  again this is sufficient for coarse interleaving but maybe not for fine*)
+
+
+Section Tracksem.
+  Context {G C:Type} (Sem: @EffectSem G C) (g:G).
+
+  Fixpoint trackstepN (n:nat) : (block -> Z -> bool) -> C -> mem -> C -> mem -> Prop :=
+    match n with
+      | O => fun U c m c' m' => (c,m) = (c',m') /\ U = (fun b z => false)
+      | S k => fun U c1 m1 c3 m3 => exists c2, exists m2, exists U1, exists U2,
+        effstep Sem g U1 c1 m1 c2 m2 /\
+        trackstepN k U2 c2 m2 c3 m3 /\
+        U = (fun b z => U1 b z || U2 b z)
+    end.
+
+  Lemma trackstepN_effstepN
+   (DET: forall c m c1 m1 U1 c2 m2 U2, effstep Sem g U1 c m c1 m1 -> 
+         effstep Sem g U2 c m c2 m2 -> (c1,m1,U1)=(c2,m2,U2)):
+  forall n c m c' m' W U,
+  trackstepN n W c m c' m' -> effstepN Sem g n U c m c' m' ->
+  U = fun b z => W b z && valid_block_dec m b.
+  Proof. induction n; simpl; intros.
+  + destruct H as [? ?]. inv H. 
+    destruct H0 as [? ?]. inv H. simpl in *; trivial.
+  + destruct H as [c1 [m1 [U1 [U2 [Estep [Tsteps HW]]]]]].
+    destruct H0 as [c1' [m1' [U1' [U2' [Estep' [Esteps HU]]]]]].
+    specialize (DET _ _ _ _ _ _ _ _ Estep' Estep). inv DET.
+    specialize (IHn _ _ _ _ _ _ Tsteps Esteps); subst.
+    extensionality b; extensionality z.
+    remember (U1 b z) as q; symmetry in Heqq. destruct q; simpl in *.
+    - exploit @effstep_valid. apply Estep. apply Heqq.
+      destruct (valid_block_dec m b); trivial; simpl in *; congruence.
+    - remember (U2 b z) as p; symmetry in Heqp. destruct p; simpl in *; [| congruence].
+      destruct (valid_block_dec m1 b); simpl; trivial.
+      destruct (valid_block_dec m b); simpl; trivial.
+      elim n0. eapply effstep_fwd. eassumption.
+      destruct (valid_block_dec m b); trivial; simpl in *; congruence.
+Qed.
+
+  Lemma trackstepN_effstep_iff:
+  forall n c m c' m',
+  (exists W, effstepN Sem g n W c m c' m') <-> (exists W, trackstepN n W c m c' m').
+  Proof. induction n; simpl; intros.
+  + split; trivial.
+  + split; intros [W [cc [mm [U1 [U2 [Estep [Steps HW]]]]]]].
+    - destruct (IHn cc mm c' m') as [X _].
+      exploit X; clear X. exists U2; trivial. intros [U T].
+      eexists; exists cc, mm; eexists; eexists. split. eassumption. 
+      split. eassumption. reflexivity. 
+    - destruct (IHn cc mm c' m') as [_ X].
+      exploit X; clear X. exists U2; trivial. intros [U T].
+      eexists; exists cc, mm; eexists; eexists. split. eassumption. 
+      split. eassumption. reflexivity.
+  Qed.
+
+  Lemma trackstepN_perm: forall n U c1 m1 c2 m2, trackstepN n U c1 m1 c2 m2 ->
+       forall b z, U b z = true -> Mem.valid_block m1 b -> Mem.perm m1 b z Cur Writable.
+  Proof. intros n.
+    induction n; simpl; intros. destruct H; subst. discriminate.
+    destruct H as [c [m [U1 [U2 [Step [StepN UU]]]]]]; subst; simpl.
+    specialize (IHn _ _ _ _ _ StepN).
+    specialize (effstep_perm _ _ _ _ _ _ _ Step b z). intros.
+    remember (U1 b z) as d.
+    destruct d; simpl in *.
+    + apply H; trivial.
+    + clear H Heqd StepN.
+      specialize (IHn _ _ H0).
+      apply effstep_corestep in Step. apply corestep_mem in Step.
+      apply perm_preserve in Step. apply Step; trivial.
+      eapply Mem.perm_implies. eapply Mem.perm_max. apply IHn. apply Step. eassumption. constructor.
+      apply IHn. apply Step. eassumption.
+  Qed. 
+
+  Lemma trackstepN_mem: forall n U c m c' m' (EF: trackstepN n U c m c' m'), mem_step m m'.
+  Proof.
+    induction n; simpl; intros.
+    + destruct EF as [EF _]; inv EF. apply mem_step_refl.
+    + destruct EF as [c1 [m2 [U1 [U2 [EF1 [EF2 _]]]]]].
+      apply IHn in EF2. clear IHn.
+      apply effstep_mem in EF1.
+      eapply mem_step_trans; eassumption.
+  Qed.
+
+  Lemma trackstepN_fwd n U c m c' m' (EF:trackstepN n U c m c' m'): mem_forward m m'.
+  Proof. apply preserve_mem. apply mem_forward_preserve.
+         eapply trackstepN_mem. apply EF.
+  Qed.
+
+  Lemma trackstepN_valid' n: forall U c1 m1 c2 m2  (Step:trackstepN n U c1 m1 c2 m2)
+        b z (EFF:U b z = true), Mem.valid_block m2 b. 
+       (*Mem.valid_block m1 b may not hold - trackstep is also tracking writes to newly allocated blocks*)
+  Proof. 
+    induction n; simpl; intros. destruct Step; subst. discriminate.
+    destruct Step as [c [m [U1 [U2 [Step [StepN UU]]]]]]; subst; simpl.
+    specialize (IHn _ _ _ _ _ StepN).
+    specialize (effstep_valid _ _ _ _ _ _ _ Step b z). intros.
+    remember (U1 b z) as d; symmetry in Heqd.
+    destruct d; simpl in *; eauto.
+    eapply trackstepN_fwd. eassumption. eapply effstep_fwd. eassumption. apply H; trivial.
+  Qed.
+
+  Lemma trackstepN_corestepN: forall n E c m c' m',
+      trackstepN n E c m c' m' -> corestepN Sem g n c m c' m'.
+  Proof. intros n.
+    induction n; intros; simpl in *.
+        apply H.
+      destruct H as [c1 [m1 [U1 [U2 [Estep [EN HE]]]]]].
+        apply effstep_corestep in Estep.
+        apply IHn in EN. exists c1, m1.
+        split; eassumption.
+  Qed.
+
+  Lemma trackstepN_unchanged: forall n U c1 m1 c2 m2,
+        trackstepN n U c1 m1 c2 m2 ->
+        Mem.unchanged_on (fun b z => U b z = false) m1 m2.
+  Proof. intros n.
+    induction n; simpl; intros.
+      destruct H. inv H. apply Mem.unchanged_on_refl.
+    rename c2 into c3. rename m2 into m3.
+    destruct H as [c2 [m2 [E1 [E2 [Step1 [Step2 HE]]]]]].
+    apply IHn in Step2; clear IHn. subst.
+    assert (FWD:= effstep_fwd _ _ _ _ _ _ _ Step1).
+    apply effstep_unchanged in Step1.
+    split; intros.
+     eapply Ple_trans; [apply Step1 | apply Step2].
+     apply orb_false_iff in H. destruct H.
+     remember (valid_block_dec m1 b) as v.
+     destruct v; simpl in *; try contradiction.
+     clear H0 Heqv.
+     split; intros. apply Step2; trivial.
+        apply (FWD _ v).
+     apply Step1; try assumption.
+
+     apply Step1; try assumption.
+       apply Step2; try assumption.
+        apply (FWD _ v).
+
+   apply orb_false_iff in H. destruct H.
+     remember (valid_block_dec m1 b) as v.
+     destruct v; simpl in *; try contradiction.
+     clear Heqv.
+     destruct Step2. rewrite unchanged_on_contents; trivial.
+       eapply Step1; try eassumption.
+       eapply Step1; try eassumption.
+     elim n0. eapply Mem.perm_valid_block; eassumption.
+  Qed.
+
+  Lemma trackstepN_perm2: forall n U c1 m1 c2 m2, trackstepN n U c1 m1 c2 m2 ->
+       forall b z, U b z = true -> Mem.perm m2 b z Cur Writable.
+  (*does not hold -- location may have been freed after the write access later*)
+  Abort. 
+
+Lemma trackstepN_trans: forall n1 n2 U1 st1 m1 st2 m2 U2 st3 m3,
+      trackstepN n1 U1 st1 m1 st2 m2 ->
+      trackstepN n2 U2 st2 m2 st3 m3 ->
+   trackstepN (n1+n2)
+        (fun b z => U1 b z || U2 b z) st1 m1 st3 m3.
+Proof. intros n1.
+induction n1; simpl.
++ intros. destruct H; subst. inv H. simpl. trivial.
++ intros. rename st3 into st4. rename m3 into m4.
+   rename st2 into st3. rename m2 into m3.
+   rename U1 into U. rename U2 into U3.
+   destruct H as [st2 [m2 [U1 [U2 [Step1 [Step2 HU]]]]]].
+   subst; simpl in *.
+   exists st2, m2, U1; simpl.
+   specialize (IHn1 _ _ _ _ _ _ _ _ _ Step2 H0).
+   clear Step2 H0.
+   eexists; split. assumption.
+   split. eassumption.
+   extensionality b; extensionality z; simpl. rewrite orb_assoc; trivial.
+Qed.
+
+Lemma trackstepN_trans': forall n1 n2 U U1 st1 m1 st2 m2 U2 st3 m3,
+      trackstepN n1 U1 st1 m1 st2 m2 ->
+      trackstepN n2 U2 st2 m2 st3 m3 ->
+      U = (fun b z => U1 b z || U2 b z) ->
+   trackstepN (n1+n2) U st1 m1 st3 m3.
+Proof. intros; subst. eapply trackstepN_trans; eassumption. Qed.
+
+  Definition trackstep_plus U c m c' m' :=
+    exists n, trackstepN (S n) U c m c' m'.
+
+  Definition trackstep_star U c m c' m' :=
+    exists n, trackstepN n U c m c' m'.
+
+  Lemma trackstep_plus_corestep_plus U c m c' m' (EFF: trackstep_plus U c m c' m'):
+        corestep_plus Sem g c m c' m'.
+  Proof. destruct EFF. apply trackstepN_corestepN in H. exists x; trivial. Qed.
+
+  Lemma trackstep_star_corestep_star U c m c' m' (EFF: trackstep_star U c m c' m'):
+        corestep_star Sem g c m c' m'.
+  Proof. destruct EFF. apply trackstepN_corestepN in H. exists x; trivial. Qed.
+
+  Lemma trackstep_plus_star : forall U c1 c2 m1 m2,
+    trackstep_plus U c1 m1 c2 m2 -> trackstep_star U c1 m1 c2 m2.
+  Proof. intros. destruct H as [n1 H1]. eexists. apply H1. Qed.
+
+  Lemma trackstep_plus_trans : forall U1 c1 c2 c3 U2 m1 m2 m3,
+    trackstep_plus U1 c1 m1 c2 m2 -> trackstep_plus U2 c2 m2 c3 m3 ->
+    trackstep_plus (fun b z => U1 b z || U2 b z) c1 m1 c3 m3.
+  Proof. intros. destruct H as [n1 H1]. destruct H0 as [n2 H2].
+    exists ((n1 + (S n2))%nat). simpl.
+    apply (trackstepN_trans (S n1) (S n2) U1 c1 m1 c2 m2 U2 c3 m3 H1 H2).
+  Qed.
+  Lemma trackstep_plus_trans' : forall U U1 c1 c2 c3 U2 m1 m2 m3,
+    trackstep_plus U1 c1 m1 c2 m2 -> trackstep_plus U2 c2 m2 c3 m3 ->
+    U = (fun b z => U1 b z || U2 b z) ->
+    trackstep_plus U c1 m1 c3 m3.
+  Proof. intros; subst. eapply trackstep_plus_trans; eassumption. Qed.
+
+  Lemma trackstep_star_plus_trans : forall U1 c1 c2 c3 U2 m1 m2 m3,
+    trackstep_star U1 c1 m1 c2 m2 -> trackstep_plus U2 c2 m2 c3 m3 ->
+    trackstep_plus (fun b z => U1 b z || U2 b z) c1 m1 c3 m3.
+  Proof. intros. destruct H as [n1 H1]. destruct H0 as [n2 H2].
+    exists ((n1 + n2)%nat).
+    specialize (trackstepN_trans n1 (S n2) U1 c1 m1 c2 m2 U2 c3 m3 H1 H2); intros H.
+    rewrite <- plus_n_Sm in H. assumption.
+  Qed.
+  Lemma trackstep_star_plus_trans' : forall U U1 c1 c2 c3 U2 m1 m2 m3,
+    trackstep_star U1 c1 m1 c2 m2 -> trackstep_plus U2 c2 m2 c3 m3 ->
+    U = (fun b z => U1 b z || U2 b z) ->
+    trackstep_plus U c1 m1 c3 m3.
+  Proof. intros; subst. eapply trackstep_star_plus_trans; eassumption. Qed.
+
+  Lemma trackstep_plus_star_trans: forall U1 c1 c2 c3 U2 m1 m2 m3,
+    trackstep_plus U1 c1 m1 c2 m2 -> trackstep_star U2 c2 m2 c3 m3 ->
+    trackstep_plus (fun b z => U1 b z || U2 b z) c1 m1 c3 m3.
+  Proof. intros. destruct H as [n1 H1]. destruct H0 as [n2 H2].
+    exists ((n1 + n2)%nat).
+    apply (trackstepN_trans _ _  U1 c1 m1 c2 m2 U2 c3 m3 H1 H2).
+  Qed.
+  Lemma trackstep_plus_star_trans': forall U U1 c1 c2 c3 U2 m1 m2 m3,
+    trackstep_plus U1 c1 m1 c2 m2 -> trackstep_star U2 c2 m2 c3 m3 ->
+    U = (fun b z => U1 b z || U2 b z) ->
+    trackstep_plus U c1 m1 c3 m3.
+  Proof. intros; subst. eapply trackstep_plus_star_trans; eassumption. Qed.
+
+  Lemma trackstep_star_trans: forall U1 c1 c2 c3 U2 m1 m2 m3,
+    trackstep_star U1 c1 m1 c2 m2 -> trackstep_star U2 c2 m2 c3 m3 ->
+    trackstep_star (fun b z => U1 b z || U2 b z) c1 m1 c3 m3.
+  Proof. intros. destruct H as [n1 H1]. destruct H0 as [n2 H2].
+    eexists.
+    eapply (trackstepN_trans _ _ U1 c1 m1 c2 m2 U2 c3 m3 H1 H2).
+  Qed.
+  Lemma trackstep_star_trans': forall U U1 c1 c2 c3 U2 m1 m2 m3,
+    trackstep_star U1 c1 m1 c2 m2 -> trackstep_star U2 c2 m2 c3 m3 ->
+    U = (fun b z => U1 b z || U2 b z) ->
+    trackstep_star U c1 m1 c3 m3.
+  Proof. intros; subst. eapply trackstep_star_trans; eassumption. Qed.
+
+  Lemma trackstep_plus_one: forall U c m c' m',
+    effstep Sem g U c m c' m' -> trackstep_plus U c m c' m'.
+  Proof. intros. exists O. simpl. exists c', m', U, (fun b z =>false).
+    intuition.
+    extensionality b; extensionality z; simpl.
+    rewrite orb_false_r. trivial.
+  Qed.
+
+  Lemma trackstep_plus_two: forall U1 c m c' m' U2 c'' m'',
+    effstep  Sem g U1 c m c' m' -> effstep Sem g U2 c' m' c'' m'' ->
+    trackstep_plus (fun b z => U1 b z || U2 b z) c m c'' m''.
+  Proof. intros.
+    exists (S O). exists c', m', U1, U2. split; trivial.
+    split; trivial. simpl.
+    exists c'', m'', U2, (fun b z =>false).
+    intuition.
+    extensionality b; extensionality z; simpl.
+    rewrite orb_false_r. trivial.
+  Qed.
+
+  Lemma trackstep_star_zero: forall c m, trackstep_star (fun b z =>false) c m c m.
+  Proof. intros. exists O. simpl. split; reflexivity. Qed.
+
+  Lemma trackstep_star_one: forall U c m c' m',
+    effstep  Sem g U c m c' m' -> trackstep_star U c m c' m'.
+  Proof. intros.
+    exists (S O). exists c', m', U, (fun b z =>false).
+    simpl; split; trivial. split. split; reflexivity.
+    extensionality b; extensionality z; simpl.
+    rewrite orb_false_r. trivial.
+  Qed.
+
+  Lemma trackstep_plus_split: forall U c m c' m',
+    trackstep_plus U c m c' m' ->
+    exists c'', exists m'', exists U1, exists U2,
+      effstep Sem g U1 c m c'' m'' /\
+      trackstep_star U2 c'' m'' c' m' /\
+      U = (fun b z => U1 b z || U2 b z).
+  Proof. intros.
+    destruct H as [n [c2 [m2 [U1 [U2 [Hstep [Hstar HU]]]]]]].
+    exists c2, m2, U1, U2. split. assumption. split; try assumption.
+    exists n. assumption.
+  Qed.
+
+  Lemma trackstep_plus_perm U c1 m1 c2 m2 (Step: trackstep_plus U c1 m1 c2 m2):
+       forall b z, U b z = true -> Mem.valid_block m1 b -> Mem.perm m1 b z Cur Writable.
+  Proof. destruct Step. eapply trackstepN_perm; eassumption. Qed.
+
+  Lemma trackstep_star_perm U c1 m1 c2 m2 (Step: trackstep_star U c1 m1 c2 m2):
+       forall b z, U b z = true -> Mem.valid_block m1 b -> Mem.perm m1 b z Cur Writable.
+  Proof. destruct Step. eapply trackstepN_perm; eassumption. Qed.
+
+  Lemma trackstep_plus_valid' U c1 m1 c2 m2 (Step: trackstep_plus U c1 m1 c2 m2):
+       forall b z, U b z = true -> Mem.valid_block m2 b.
+  Proof. destruct Step. eapply trackstepN_valid'; eassumption. Qed.
+
+  Lemma trackstep_star_valid' U c1 m1 c2 m2 (Step: trackstep_star U c1 m1 c2 m2):
+       forall b z, U b z = true -> Mem.valid_block m2 b.
+  Proof. destruct Step. eapply trackstepN_valid'; eassumption. Qed.
+
+  Lemma trackstep_star_mem U c m c' m' (EF: trackstep_star U c m c' m'): mem_step m m'.
+  Proof. destruct EF as [n H].
+      eapply trackstepN_mem; eassumption.
+  Qed.
+
+  Lemma trackstep_plus_mem U c m c' m' (EF: trackstep_plus U c m c' m'): mem_step m m'.
+  Proof. destruct EF as [n H].
+      eapply trackstepN_mem; eassumption.
+  Qed.
+
+  Lemma trackstep_plus_fwd U c m c' m' (EF: trackstep_plus U c m c' m'): mem_forward m m'.
+  Proof. apply preserve_mem. apply mem_forward_preserve.
+         eapply trackstep_plus_mem. apply EF.
+  Qed.
+  Lemma trackstep_star_fwd U c m c' m' (EF: trackstep_star U c m c' m'): mem_forward m m'.
+  Proof. apply preserve_mem. apply mem_forward_preserve.
+         eapply trackstep_star_mem. apply EF.
+  Qed.
+
+  Lemma trackstep_star_unchanged U c1 m1 c2 m2 (T: trackstep_star U c1 m1 c2 m2):
+        Mem.unchanged_on (fun b z => U b z = false) m1 m2.
+  Proof. destruct T. apply trackstepN_unchanged in H; trivial. Qed.
+
+  Lemma trackstep_plus_unchanged U c1 m1 c2 m2 (T: trackstep_plus U c1 m1 c2 m2):
+        Mem.unchanged_on (fun b z => U b z = false) m1 m2.
+  Proof. destruct T. apply trackstepN_unchanged in H; trivial. Qed.
+
+End Tracksem.
+(*
+Require Import VST.concurrency.paco.src.paco.
+
+Section TRACKDIV.
+  Context {G C:Type} (Sem: @EffectSem G C) (g:G). 
+
+  CoInductive trackdiv: C -> mem -> (block -> Z -> bool) -> Prop :=
+  | Trackdiv: forall c m W c1 m1 U V, effstep Sem g W c m c1 m1 -> trackdiv c1 m1 U ->
+              V =(fun b z => W b z || U b z) ->
+            trackdiv c m V.
+
+  Variable R: C -> mem -> (block -> Z -> bool) -> Prop.
+
+  Hypothesis TrackCase : forall c m V, R c m V -> 
+    exists U W c1 m1, effstep Sem g W c m c1 m1 /\ trackdiv c1 m1 U  /\ 
+                      V = (fun b z => W b z || U b z).
+
+  Theorem track_coind : forall c m V, R c m V -> trackdiv c m V. 
+  Proof. cofix; intros. clear track_coind. 
+     destruct (TrackCase _ _ _ H) as [U [W [c1 [m1 [Step [Steps HV]]]]]]; subst.
+     econstructor; eauto.
+  Qed.
+
+  Lemma trackdiv_perm: forall c m W (Step: trackdiv c m W) b z,
+      W b z = true -> Mem.valid_block m b -> Mem.perm m b z Cur Writable.
+  Proof. intros. pinversion Step. punfold Step. pcofix Step. intros c m W Step. inversion Step; subst. cofix. Step. inv Step. rename W0 into W.
+    remember (W b z) as w; symmetry in Heqw; destruct w; simpl in H.
+  + eapply effstep_perm; eauto.
+  + apply effstep_unchanged in H1. apply H1; trivial; clear H1. 
+     Check track_coind.
+
+End TRACKDIV.
+*)
+
+Inductive MidStepTrackResult {C:Type} :=
+  MST_Ext: C -> mem -> (block -> Z -> bool) -> external_function -> list val -> MidStepTrackResult
+| MST_Ret: C -> mem -> (block -> Z -> bool) -> val -> MidStepTrackResult
+| MST_Div: (block -> Z -> Prop) -> MidStepTrackResult. (*DO track written locations*)
+
+Inductive midstepT {G C} (SEM : @EffectSem G C) g (c:C) (m:mem):
+          @MidStepTrackResult C -> Prop:=
+  mst_ext: forall c' m' W f args,
+          trackstep_star SEM g W c m c' m' ->
+          at_external SEM c' = Some (f,args) ->
+          midstepT SEM g c m (MST_Ext c' m' W f args)
+| mst_ret: forall c' m' W v,
+          trackstep_star SEM g W c m c' m' ->
+          halted SEM c' = Some v ->
+          midstepT SEM g c m (MST_Ret c' m' W v)
+(*| mst_div: forall W, trackdiv SEM g c m W ->
+           midstepT SEM g c m (MST_Div W).*)
+| mst_div: forall W (U : nat -> block -> Z -> bool)
+               (ci: nat -> C) (mi: nat -> mem)
+               (Steps: forall i, trackstepN SEM g i (U i) c m (ci i) (mi i))
+               (HW: forall b z, W b z <-> exists i, U i b z = true)
+               (H: (ci O, mi O) = (c,m)),
+          midstepT SEM g c m (MST_Div W).
+(*Alternative definition of last case using individual tracksteps:
+| mst_div: forall W (U : nat -> block -> Z -> bool)
+               (ci: nat -> C) (mi: nat -> mem)
+               (Steps: forall i, trackstepN SEM g 1 (U i) (ci i) (mi i) (ci (S i)) (mi (S i)))
+               (HW: forall b z, W b z = true <-> exists i, U i b z = true)
+               (H: (ci O, mi O) = (c,m)),
+          midstepT SEM g c m (MST_Div W).*)
+
+Definition Wset {C} (R:@MidStepTrackResult C) : (block -> Z -> Prop) :=
+  match R with
+    MST_Ext _ _ W _ _ => (fun b z => W b z = true)
+  | MST_Ret _ _ W _ => (fun b z => W b z = true)
+  | MST_Div W => W
+  end.
+
+  Lemma midstepT_perm {G C} (SEM : @EffectSem G C) g c1 m1 R (Step: midstepT SEM g c1 m1 R):
+       forall b z, Wset R b z -> Mem.valid_block m1 b -> Mem.perm m1 b z Cur Writable.
+  Proof. destruct Step; simpl.
+    + eapply trackstep_star_perm; eassumption.
+    + eapply trackstep_star_perm; eassumption.
+    + intros. apply HW in H0. destruct H0 as [i I].
+      eapply trackstepN_perm; eauto. 
+  Qed.
+
+Definition MST_unchanged_on {C} m (A: @MidStepTrackResult C) :=
+  match A with
+    MST_Ext _ m' W _ _ => Mem.unchanged_on (fun b z => W b z = false) m m'
+  | MST_Ret _ m' W  _ => Mem.unchanged_on (fun b z => W b z = false) m m'
+  | MST_Div _ => True
+  end.
+
+  Lemma midstepT_unchanged {G C} (SEM : @EffectSem G C) g c1 m1 R (Step: midstepT SEM g c1 m1 R):
+        MST_unchanged_on m1 R.
+  Proof. inv Step; simpl; trivial; eapply trackstep_star_unchanged; eassumption. Qed.
+
+Lemma corestepN_midstepT_atExt {G C} (SEM : @EffectSem G C) g: forall n c1 m1 c2 m2 f args,
+   corestepN SEM g n c1 m1 c2 m2 -> at_external SEM c2 = Some (f,args) ->
+   exists W, midstepT SEM g c1 m1 (MST_Ext c2 m2 W f args) /\
+             forall b z, W b z = true -> Mem.valid_block m1 b -> Mem.perm m1 b z Cur Writable.
+Proof. intros.
+  apply corestepN_effstepN in H. destruct H as [U EFF].
+  destruct (trackstepN_effstep_iff SEM g n c1 m1 c2 m2) as [X _].
+  exploit X; clear X. eexists; eassumption. intros [W HW]. clear EFF.
+  eexists; split. econstructor. exists n; apply HW. trivial.
+  eapply trackstepN_perm; eassumption.
+Qed. 
+
+Lemma corestepN_midstepT_Ret {G C} (SEM : @EffectSem G C) g: forall n c1 m1 c2 m2 v,
+   corestepN SEM g n c1 m1 c2 m2 -> halted SEM c2 = Some v ->
+   exists W, midstepT SEM g c1 m1 (MST_Ret c2 m2 W v) /\
+             forall b z, W b z = true -> Mem.valid_block m1 b -> Mem.perm m1 b z Cur Writable.
+Proof. intros.
+  apply corestepN_effstepN in H. destruct H as [U EFF].
+  destruct (trackstepN_effstep_iff SEM g n c1 m1 c2 m2) as [X _].
+  exploit X; clear X. eexists; eassumption. intros [W HW]. clear EFF.
+  eexists; split. econstructor. exists n; apply HW. trivial.
+  eapply trackstepN_perm; eassumption.
+Qed.
+
+Require Import Coq.Logic.ChoiceFacts.
+
+(*Of course, some writes in the diverging exection (DE) may be to locations in 
+blocks that are only allocated during DE.
+But these locations are not shared with other threads (since DE does not make external calls).
+So they can;t participate in races, so coarse-to-fine-proof should be ok.
+Also not that the shared/nonshared info of locations in blocks valid in m1 never changes, 
+again because DE doe not contain lock/unlock calls.*)
+Lemma corestepN_midstepT_Div {G C} (FCC: FunctionalChoice_on nat C)
+   (FCM: FunctionalChoice_on nat mem) (FCW: FunctionalChoice_on nat (block -> Z -> bool))
+   (SEM : @EffectSem G C) g: forall c1 m1,
+   (forall n, exists c2 m2, corestepN SEM g n c1 m1 c2 m2) -> 
+   exists W, midstepT SEM g c1 m1 (MST_Div W) /\
+             forall b z, W b z -> Mem.valid_block m1 b -> Mem.perm m1 b z Cur Writable.
+Proof. intros.
+  assert (ESTEPS: forall n : nat,
+    exists (c2 : C) (m2 : mem) Wn, effstepN SEM g n Wn c1 m1 c2 m2).
+  { intros. destruct (H n) as [c2 [m2 STEP]]. exists c2, m2.
+    apply corestepN_effstepN in STEP; trivial. }
+  clear H.
+  destruct (FCC _ ESTEPS) as [fC HC]; clear ESTEPS.
+  destruct (FCM _ HC) as [fM HM]; clear HC.
+  assert (HT: forall n, exists W, trackstepN SEM g n W c1 m1 (fC n) (fM n)).
+  { intros. apply (trackstepN_effstep_iff SEM g n c1 m1 (fC n) (fM n)); trivial. } 
+  destruct (FCW _ HT) as [fU HU]; clear HT HM.
+  exists (fun b z => exists i, fU i b z = true); split.
+  + econstructor. eassumption. intros; split; trivial.
+    specialize (HU O). destruct HU as [Q _]; rewrite Q; trivial.
+  + intros. destruct H as [i I]. specialize (HU i).
+    eapply trackstepN_perm; eassumption.
+Qed.
+(*
+------
+Inductive MidStepTrackResult {C:Type} :=
+  MST_Ext: C -> mem -> (block -> Z -> bool) -> external_function -> list val -> MidStepTrackResult
+| MST_Ret: C -> mem -> (block -> Z -> bool) -> val -> MidStepTrackResult
+| MST_Div: (block -> Z -> bool) -> MidStepTrackResult. (*DO track written locations*)
+
+Inductive midstepT {G C} (SEM : @EffectSem G C) g (c:C) (m:mem):
+          @MidStepTrackResult C -> Prop:=
+  mst_ext: forall c' m' W f args,
+          trackstep_star SEM g W c m c' m' ->
+          at_external SEM c' = Some (f,args) ->
+          midstepT SEM g c m (MST_Ext c' m' W f args)
+| mst_ret: forall c' m' W v,
+          trackstep_star SEM g W c m c' m' ->
+          halted SEM c' = Some v ->
+          midstepT SEM g c m (MST_Ret c' m' W v)
+| mst_div: forall W (U : nat -> block -> Z -> bool)
+               (ci: nat -> C) (mi: nat -> mem)
+               (Steps: forall i, trackstepN SEM g i (U i) c m (ci i) (mi i))
+               (HW: forall b z, W b z = true <-> exists i, U i b z = true)
+               (H: (ci O, mi O) = (c,m)),
+          midstepT SEM g c m (MST_Div W).
+(*Alternative definition of last case unsing individual tracksteps:
+| mst_div: forall W (U : nat -> block -> Z -> bool)
+               (ci: nat -> C) (mi: nat -> mem)
+               (Steps: forall i, trackstepN SEM g 1 (U i) (ci i) (mi i) (ci (S i)) (mi (S i)))
+               (HW: forall b z, W b z = true <-> exists i, U i b z = true)
+               (H: (ci O, mi O) = (c,m)),
+          midstepT SEM g c m (MST_Div W).*)
+
+Definition Wset {C} (R:@MidStepTrackResult C) : (block -> Z -> bool) :=
+  match R with
+    MST_Ext _ _ W _ _ => W
+  | MST_Ret _ _ W _ => W
+  | MST_Div W => W
+  end.
+
+  Lemma midstepT_perm {G C} (SEM : @EffectSem G C) g c1 m1 R (Step: midstepT SEM g c1 m1 R):
+       forall b z, Wset R b z = true -> Mem.valid_block m1 b -> Mem.perm m1 b z Cur Writable.
+  Proof. destruct Step; simpl.
+    + eapply trackstep_star_perm; eassumption.
+    + eapply trackstep_star_perm; eassumption.
+    + intros. apply HW in H0. destruct H0 as [i I].
+      eapply trackstepN_perm; eauto. 
+  Qed.
+
+Definition MST_unchanged_on {C} m (A: @MidStepTrackResult C) :=
+  match A with
+    MST_Ext _ m' W _ _ => Mem.unchanged_on (fun b z => W b z = false) m m'
+  | MST_Ret _ m' W  _ => Mem.unchanged_on (fun b z => W b z = false) m m'
+  | MST_Div _ => True
+  end.
+
+  Lemma midstepT_unchanged {G C} (SEM : @EffectSem G C) g c1 m1 R (Step: midstepT SEM g c1 m1 R):
+        MST_unchanged_on m1 R.
+  Proof. inv Step; simpl; trivial; eapply trackstep_star_unchanged; eassumption. Qed.
+
+Lemma corestepN_midstepT_atExt {G C} (SEM : @EffectSem G C) g: forall n c1 m1 c2 m2 f args,
+   corestepN SEM g n c1 m1 c2 m2 -> at_external SEM c2 = Some (f,args) ->
+   exists W, midstepT SEM g c1 m1 (MST_Ext c2 m2 W f args) /\
+             forall b z, W b z = true -> Mem.valid_block m1 b -> Mem.perm m1 b z Cur Writable.
+Proof. intros.
+  apply corestepN_effstepN in H. destruct H as [U EFF].
+  destruct (trackstepN_effstep_iff SEM g n c1 m1 c2 m2) as [X _].
+  exploit X; clear X. eexists; eassumption. intros [W HW]. clear EFF.
+  eexists; split. econstructor. exists n; apply HW. trivial.
+  eapply trackstepN_perm; eassumption.
+Qed. 
+
+Lemma corestepN_midstepT_Ret {G C} (SEM : @EffectSem G C) g: forall n c1 m1 c2 m2 v,
+   corestepN SEM g n c1 m1 c2 m2 -> halted SEM c2 = Some v ->
+   exists W, midstepT SEM g c1 m1 (MST_Ret c2 m2 W v) /\
+             forall b z, W b z = true -> Mem.valid_block m1 b -> Mem.perm m1 b z Cur Writable.
+Proof. intros.
+  apply corestepN_effstepN in H. destruct H as [U EFF].
+  destruct (trackstepN_effstep_iff SEM g n c1 m1 c2 m2) as [X _].
+  exploit X; clear X. eexists; eassumption. intros [W HW]. clear EFF.
+  eexists; split. econstructor. exists n; apply HW. trivial.
+  eapply trackstepN_perm; eassumption.
+Qed. 
+
+Require Import Coq.Logic.ChoiceFacts.
+
+Lemma corestepN_midstepT_Div {G C} (FCC: FunctionalChoice_on nat C)
+   (FCM: FunctionalChoice_on nat mem) (FCW: FunctionalChoice_on nat (block -> Z -> bool))
+   (FF: FunctionalRelReification_on (block * Z) (block -> Z -> bool))
+   (SEM : @EffectSem G C) g: forall c1 m1,
+   (forall n, exists c2 m2, corestepN SEM g n c1 m1 c2 m2) -> 
+   exists W, midstepT SEM g c1 m1 (MST_Div W) /\
+             forall b z, W b z = true -> Mem.valid_block m1 b -> Mem.perm m1 b z Cur Writable.
+Proof. intros.
+  assert (ESTEPS: forall n : nat,
+    exists (c2 : C) (m2 : mem) Wn, effstepN SEM g n Wn c1 m1 c2 m2).
+  { intros. destruct (H n) as [c2 [m2 STEP]]. exists c2, m2.
+    apply corestepN_effstepN in STEP; trivial. }
+  clear H.
+  destruct (FCC _ ESTEPS) as [fC HC]; clear ESTEPS.
+  destruct (FCM _ HC) as [fM HM]; clear HC.
+  assert (HT: forall n, exists W, trackstepN SEM g n W c1 m1 (fC n) (fM n)).
+  { intros. apply (trackstepN_effstep_iff SEM g n c1 m1 (fC n) (fM n)); trivial. } 
+  destruct (FCW _ HT) as [fU HU]; clear HT HM. 
+  assert (HW: exists W: block -> Z -> bool, forall b z, W b z = true <-> exists i, fU i b z = true).
+  { clear HU g c1 m1 fC fM.
+Check Mem.unchanged_on.
+    destruct (FF (fun bz f => exists i, fU i (fst bz) (snd bz) = true)).
+    + intros [b z]. simpl. admit.
+    + }
+  destruct HW as [W HW].
+  exists W; split.
+  + econstructor. eassumption. trivial.
+    specialize (HU O). destruct HU as [Q _]; rewrite Q; trivial.
+  + intros. apply HW in H. destruct H as [i I]. specialize (HU i).
+    eapply trackstepN_perm; eassumption.
+Qed. 
+  
+------
+Definition addeffect {C} m (U:block -> Z -> bool) (R: @MidStepEffectResult C) :=
+  match R with
+    MSE_Ext c' m' W f args => MSE_Ext c' m' (fun b z => U b z || W b z  && valid_block_dec m b)  f args
+  | MSE_Ret c' m' W v => MSE_Ret c' m' (fun b z => U b z || W b z  && valid_block_dec m b) v
+  | MSE_Div => MSE_Div
+  end.
+
+Lemma midtepE_preserves_trackstep_rev {G C} (SEM : @EffectSem G C) g:
+   forall c m  U c' m', trackstep SEM g U c m c' m' ->
+   forall R, midstepE SEM g c' m' R -> midstepE SEM g c m (addeffect m U R).
+Proof. intros. inv H0.
++ constructor; trivial. destruct H1 as [n N].
+  exists (S n), c', m'; eexists; eexists; split. eassumption.
+  split. eassumption. trivial.
++ constructor; trivial. destruct H1 as [n N].
+  exists (S n), c', m'; eexists; eexists; split. eassumption.
+  split. eassumption. trivial.
++ constructor; intros. destruct n. 
+  - eexists; eexists; reflexivity. 
+  - simpl. destruct (H1 n) as [cc [mm CM]].
+    apply effstep_corestep in H.
+    exists cc, mm, c', m'. split; trivial.
+Qed. 
+
+Definition minuseffect {C} m (U:block -> Z -> bool) (R: @MidStepEffectResult C) :=
+  match R with
+    MSE_Ext c' m' W f args => MSE_Ext c' m' (fun b z => W b z && valid_block_dec m b)  f args
+  | MSE_Ret c' m' W v => MSE_Ret c' m' (fun b z => U b z || W b z  && valid_block_dec m b) v
+  | MSE_Div => MSE_Div
+  end.
+
+Lemma midtepE_preserves_effstep {G C} (SEM : @EffectSem G C) g
+   (DET: forall c m c1 m1 U1 c2 m2 U2, effstep SEM g U1 c m c1 m1 -> 
+         effstep SEM g U2 c m c2 m2 -> (c1,m1,U1)=(c2,m2,U2)):
+   forall c m U c' m', effstep SEM g U c m c' m' ->
+   forall R, midstepE SEM g c m R -> 
+          midstepE SEM g c' m' (minuseffect 
+Proof. intros. destruct R. simpl.
++ rename b into V. simpl in H0. inv H0. constructor; trivial. 
+  remember (fun (b : block) (z : Z) => U b z || V b z && valid_block_dec m b) as W.
+  generalize dependent V. 
+  destruct H3 as [n N]. generalize dependent W. 
+  destruct n; simpl in *; intros.
+  - destruct N as [N1 N2]. inv N1.
+    apply effstep_corestep in H.
+    apply corestep_not_at_external in H. congruence.
+  - destruct N as [cc [mm [U1 [U2 [STEP [STEPS HU]]]]]].
+    specialize (DET _ _ _ _ _ _ _ _ H STEP); inv DET.
+    exists n; trivial.
++ constructor; trivial.
+  destruct H1 as [n N].
+  induction n; simpl in *.
+  - inv N. apply corestep_not_halted in H. congruence.
+  - destruct N as [cc [mm [STEP STEPS]]]. specialize (DET _ _ _ _ _ _ H STEP); inv DET.
+    exists n; trivial.
++ constructor; intros. destruct (H1 (S n)) as [cc [mm MM]]; clear H1; simpl in MM.
+  destruct MM as [c1 [m1 [STEP STEPS]]].
+  specialize (DET _ _ _ _ _ _ H STEP); inv DET.
+  exists cc, mm; trivial.
+Qed.
+
+Definition addeffect {C} m (U:block -> Z -> bool) (R: @MidStepEffectResult C) :=
+  match R with
+    MSE_Ext c' m' W f args => MSE_Ext c' m' (fun b z => U b z || W b z  && valid_block_dec m b)  f args
+  | MSE_Ret c' m' W v => MSE_Ret c' m' (fun b z => U b z || W b z  && valid_block_dec m b) v
+  | MSE_Div => MSE_Div
+  end.
+
+Lemma midtepE_preserves_effstep_rev {G C} (SEM : @EffectSem G C) g:
+   forall c m  U c' m', effstep SEM g U c m c' m' ->
+   forall R, midstepE SEM g c' m' R -> midstepE SEM g c m (addeffect m U R).
+Proof. intros. inv H0.
++ constructor; trivial. destruct H1 as [n N].
+  exists (S n), c', m'; eexists; eexists; split. eassumption.
+  split. eassumption. trivial.
++ constructor; trivial. destruct H1 as [n N].
+  exists (S n), c', m'; eexists; eexists; split. eassumption.
+  split. eassumption. trivial.
++ constructor; intros. destruct n. 
+  - eexists; eexists; reflexivity. 
+  - simpl. destruct (H1 n) as [cc [mm CM]].
+    apply effstep_corestep in H.
+    exists cc, mm, c', m'. split; trivial.
+Qed. 
+
+Lemma midtepE_preserves_effstep {G C} (SEM : @EffectSem G C) g
+   (DET: forall c m c1 m1 U1 c2 m2 U2, effstep SEM g U1 c m c1 m1 -> 
+         effstep SEM g U2 c m c2 m2 -> (c1,m1,U1)=(c2,m2,U2)):
+   forall c m U c' m', effstep SEM g U c m c' m' ->
+   forall R, midstepE SEM g c m (addeffect m U R) -> 
+          midstepE SEM g c' m' R.
+Proof. intros. destruct R. simpl.
++ rename b into V.  simpl in H0. inv H0. constructor; trivial. 
+  remember (fun (b : block) (z : Z) => U b z || V b z && valid_block_dec m b) as W.
+  generalize dependent V. 
+  destruct H3 as [n N]. generalize dependent W. 
+  destruct n; simpl in *; intros.
+  - destruct N as [N1 N2]. inv N1.
+    apply effstep_corestep in H.
+    apply corestep_not_at_external in H. congruence.
+  - destruct N as [cc [mm [U1 [U2 [STEP [STEPS HU]]]]]].
+    specialize (DET _ _ _ _ _ _ _ _ H STEP); inv DET.
+    exists n; trivial.
++ constructor; trivial.
+  destruct H1 as [n N].
+  induction n; simpl in *.
+  - inv N. apply corestep_not_halted in H. congruence.
+  - destruct N as [cc [mm [STEP STEPS]]]. specialize (DET _ _ _ _ _ _ H STEP); inv DET.
+    exists n; trivial.
++ constructor; intros. destruct (H1 (S n)) as [cc [mm MM]]; clear H1; simpl in MM.
+  destruct MM as [c1 [m1 [STEP STEPS]]].
+  specialize (DET _ _ _ _ _ _ H STEP); inv DET.
+  exists cc, mm; trivial.
+Qed.
+*)
