sepcomp/simulations.v
@@ -18,6 +18,47 @@ Require Import VST.sepcomp.reach.
 Require Export VST.sepcomp.globalSep.
 Require Import VST.sepcomp.semantics_lemmas.
 
+Goal forall F1 V1 C1 (Sem1 : @EffectSem (Genv.t F1 V1) C1)
+     ge1 U1 st1 m1 st1' m1' b1 z,
+     effstep Sem1 ge1 U1 st1 m1 st1' m1' -> U1 b1 z = true ->
+     Mem.perm m1 b1 z Max Nonempty.
+Proof. intros. eapply Mem.perm_implies. 
+  - apply Mem.perm_cur. eapply (effstep_perm Sem1); eassumption.
+  - constructor.
+Qed.
+
+(*In case we decide to eliminate MS_Div we can simplify the following 
+2 definitions to 
+MSR_locally_allocated mu mu' m1 m2 A1 A2 := SM_locally_allocated mu mu' m1 m2 (mem_of A1) (mem_of A2)
+and
+MSR_mem_unchanged_on P m A := Mem.unchanged_on P m (mem_of A)
+where mem_of is the obvious projection function*)
+Definition MSR_locally_allocated {C1 C2} (mu mu' : SM_Injection) (m1 m2 : mem) 
+           (A1: @MidStepResult C1 mem) (A2: @MidStepResult C2 mem):=
+match A1, A2 with
+  MS_Ext _ m1' _ _, MS_Ext _ m2' _ _ => sm_locally_allocated mu mu' m1 m2 m1' m2'
+| MS_Ret _ m1' _,  MS_Ret _ m2' _ => sm_locally_allocated mu mu' m1 m2 m1' m2'
+| _, _ => True
+end.
+
+Definition MSR_unchanged_on {C} P m (A: @MidStepResult C mem) :=
+  match A with
+    MS_Ext _ m' _ _ => Mem.unchanged_on P m m'
+  | MS_Ret _ m' _ => Mem.unchanged_on P m m'
+  | _ => True
+  end.
+
+(*This definition aims to be the mirrored version of local_out_of_reach.
+  In particular, including mem_unchange_on (extern_out_of_reach nu m1) m2 m2' in 
+  match_midstep should (fingers crossed) suffice for establishing the caller's
+  condition mem_unchanged_on (local_out_of_reach nu m1) m2 m2' 
+  of clause matchafter_external*)
+Definition extern_out_of_reach mu (m : mem) (b : block) (ofs : Z): Prop :=
+  extBlocksTgt mu b = true /\
+  forall b0 delta, extern_of mu b0 = Some (b, delta) ->
+                  (~ Mem.perm m b0 (ofs - delta) Max Nonempty \/
+                   frgnBlocksSrc mu b0 = false).
+
 (** * Structured Simulations *)
 
 Module SM_simulation. Section SharedMemory_simulation_inject.
@@ -95,6 +136,35 @@ Lemma CS2_RDO_star: forall c m c' m', corestep_star Sem2 ge2 c m c' m' ->
                   RDOnly_fwd m m' (ReadOnlyBlocks ge2).
 Proof. intros. destruct H. eapply CS2_RDO_N; eassumption. Qed.
 *)
+
+(*matchstate to be instantiated by match_state cd below*)
+Definition MSR_relate matchstate mu (A: @MidStepResult C1 mem)
+    (B: @MidStepResult C2 mem):=
+match A, B with
+  MS_Ext c1 m1 f1 vals1, MS_Ext c2 m2 f2 vals2 =>
+       Mem.inject (as_inj mu) m1 m2 /\ f1=f2
+       /\ mem_respects_readonly ge1 m1 /\ mem_respects_readonly ge2 m2
+       /\ Forall2 (val_inject (restrict (as_inj mu) (vis mu))) vals1 vals2
+       /\ forall
+       (pubSrc' pubTgt' : block -> bool)
+       (pubSrcHyp : pubSrc' =
+                  (fun b : block =>
+                  locBlocksSrc mu b && REACH m1 (exportedSrc mu vals1) b))
+       (pubTgtHyp: pubTgt' =
+                  (fun b : block =>
+                  locBlocksTgt mu b && REACH m2 (exportedTgt mu vals2) b))
+       nu (Hnu: nu = (replace_locals mu pubSrc' pubTgt')),
+       (*MSR_relate nu (MS_Ext c1 m1 f1 vals1) (MS_Ext c2 m2 f2 vals2)*)
+       matchstate nu c1 m1 c2 m2
+       /\ Mem.inject (shared_of nu) m1 m2
+| MS_Ret c1 m1 v1, MS_Ret c2 m2 v2 => 
+        Mem.inject (as_inj mu) m1 m2
+        /\ mem_respects_readonly ge1 m1 /\ mem_respects_readonly ge2 m2
+        /\ val_inject (restrict (as_inj mu) (vis mu)) v1 v2
+| MS_Div, MS_Div => True 
+| _, _ => False
+end.
+
 Record SM_simulation_inject := {
   (** The type of auxiliary data used to model stuttering. *)
   core_data : Type
@@ -146,6 +216,161 @@ Record SM_simulation_inject := {
     forall d mu c1 m1 c2 m2,
     match_state d mu c1 m1 c2 m2 ->
     sm_valid mu m1 m2
+
+(*Unifies corestep_diagram (incl step-star stuff), core_atExternal, and core_halted*)
+; match_midstep :
+    forall d mu c1 m1 c2 m2 A1,
+    match_state d mu c1 m1 c2 m2 ->
+    midstep Sem1 ge1 c1 m1 A1 ->
+    exists A2 cd' mu', 
+      midstep Sem2 ge2 c2 m2 A2
+      /\ intern_incr mu mu'
+      /\ globals_separate ge2 mu mu'
+      /\ MSR_locally_allocated mu mu' m1 m2 A1 A2 (*replaces sm_locally_allocated mu mu' m1 m2 m1' m2'*)
+      /\ MSR_relate (match_state cd') mu' A1 A2
+      /\ (MSR_unchanged_on (fun b z => vis mu b = false) m1 A1 ->
+          MSR_unchanged_on (extern_out_of_reach mu m1) m2 A2)
+      (*TODO: do we actually still need the indices cd/cd'? If yes, probably insert core_ord cd' cd clause*)
+
+(*TODO: reformulate afterExtcall*)
+}.
+
+End SharedMemory_simulation_inject.
+
+Module TRANSITIVITY. Section TRANS.
+
+Inductive sem_compose_ord_eq_eq {D12 D23:Type}
+  (ord12: D12 -> D12 -> Prop) (ord23: D23 -> D23 -> Prop) (C2:Type):
+  (D12 * option C2 * D23) ->  (D12 * option C2 * D23) ->  Prop :=
+| sem_compose_ord1 :
+  forall (d12 d12':D12) (c2:C2) (d23:D23),
+    ord12 d12 d12' -> sem_compose_ord_eq_eq ord12 ord23 C2 (d12,Some c2,d23) (d12',Some c2,d23)
+| sem_compose_ord2 :
+  forall (d12 d12':D12) (c2 c2':C2) (d23 d23':D23),
+    ord23 d23 d23' -> sem_compose_ord_eq_eq ord12 ord23 C2 (d12,Some c2,d23) (d12',Some c2',d23').
+
+Lemma well_founded_sem_compose_ord_eq_eq: forall {D12 D23:Type}
+  (ord12: D12 -> D12 -> Prop) (ord23: D23 -> D23 -> Prop)  (C2:Type)
+  (WF12: well_founded ord12) (WF23: well_founded ord23),
+  well_founded (sem_compose_ord_eq_eq ord12 ord23 C2).
+Proof.
+  intros. intro. destruct a as [[d12 c2] d23].
+  revert d12.
+  destruct c2.
+  2: constructor; intros. 2: inv H.
+  revert c.
+  induction d23 using (well_founded_induction WF23).
+  intros.
+  induction d12 using (well_founded_induction WF12).
+  constructor; intros. inv H1.
+  generalize (H0 d0). simpl. intros.
+  apply H1. auto.
+  generalize (H d1).
+  intros.
+  specialize H1. auto.
+Qed.
+
+Definition compose_sm (mu1 mu2 : SM_Injection) : SM_Injection :=
+ Build_SM_Injection
+   (locBlocksSrc mu1) (locBlocksTgt mu2)
+   (pubBlocksSrc mu1) (pubBlocksTgt mu2)
+   (compose_meminj (local_of mu1) (local_of mu2))
+   (extBlocksSrc mu1) (extBlocksTgt mu2)
+   (frgnBlocksSrc mu1) (frgnBlocksTgt mu2)
+   (compose_meminj (extern_of mu1) (extern_of mu2)).
+
+Context
+  {F1 V1 C1 F2 V2 C2 F3 V3 C3: Type}
+  (Sem1 : @EffectSem (Genv.t F1 V1) C1)
+  (Sem2 : @EffectSem (Genv.t F2 V2) C2)
+  (Sem3 : @EffectSem (Genv.t F3 V3) C3)
+  (ge1 : Genv.t F1 V1)
+  (ge2 : Genv.t F2 V2)
+  (ge3 : Genv.t F3 V3).
+
+Variable SIM12:SM_simulation_inject Sem1 Sem2 ge1 ge2.
+Definition CoreData12:= core_data _ _ _ _ SIM12.
+Definition CoreOrd12:= core_ord _ _ _ _ SIM12.
+Definition MatchState12:= match_state _ _ _ _ SIM12.
+
+Variable SIM23:SM_simulation_inject Sem2 Sem3 ge2 ge3.
+Definition CoreData23:= core_data _ _ _ _ SIM23.
+Definition CoreOrd23:= core_ord _ _ _ _ SIM23.
+Definition MatchState23:= match_state _ _ _ _ SIM23.
+
+Definition coreData:Type  :=
+       core_data Sem1 Sem2 ge1 ge2 SIM12 * option C2 *
+       core_data Sem2 Sem3 ge2 ge3 SIM23.
+
+Definition CoreOrd:= Relation_Operators.clos_trans _ (sem_compose_ord_eq_eq CoreOrd12 CoreOrd23 C2).
+
+Check (sem_compose_ord_eq_eq CoreOrd12 CoreOrd23 C2).
+
+Definition MatchState (d:coreData) (mu: SM_Injection) (c1:C1)(m1:mem)(c3:C3)(m3:mem): Prop :=
+      match d with (d1,X,d2) =>
+        exists c2, exists m2, exists mu1, exists mu2,
+          X=Some c2 /\ mu = compose_sm mu1 mu2 /\
+          MatchState12 d1 mu1 c1 m1 c2 m2 /\ MatchState23 d2 mu2 c2 m2 c3 m3
+      end.
+
+Lemma Transitivity: SM_simulation_inject Sem1 Sem3 ge1 ge3.
+Proof.
+eapply (Build_SM_simulation_inject Sem1 Sem3 ge1 ge3 coreData MatchState).
++ eapply well_founded_sem_compose_ord_eq_eq.
+  apply (core_ord_wf Sem1 Sem2 ge1 ge2 SIM12).
+  apply (core_ord_wf Sem2 Sem3 ge2 ge3 SIM23).
++ admit.
++ admit.
++ admit.
++ admit.
++ admit.
++ admit.
++ (*corediagram*) intros. rename c2 into c3. rename m2 into m3.
+  destruct d as [[d12 X] d23]. simpl in H.
+  destruct H as [c2 [m2 [mu12 [mu23 [? [? [MS12 MS23]]]]]]]; subst.
+  destruct (match_midstep _ _ _ _ SIM12 _ _ _ _ _ _ _ MS12 H0)
+   as [A2 [cd2 [mu12' [STEP2 [INC12 [SEP12 [LOCALLOC12 [REL12 UNCH2]]]]]]]].
+  simpl in *.
+  destruct (match_midstep _ _ _ _ SIM23 _ _ _ _ _ _ _ MS23 STEP2)
+   as [A3 [cd3 [mu23' [STEP3 [INC23 [SEP23 [LOCALLOC23 [REL23 UNCH3]]]]]]]].
+  exists A3, (cd2, Some c2, cd3), (compose_sm mu12' mu23'). split; trivial.
+  split. admit.
+  split. admit.
+  split. admit.
+  split. admit.
+  intros. clear - REL12 REL23 UNCH2 UNCH3 H.
+  unfold extern_out_of_reach; simpl.
+  destruct A3; simpl in *; trivial.
+  - destruct A2; try contradiction. destruct A1; try contradiction.
+    simpl in *. clear REL12 REL23.
+    exploit UNCH2; clear UNCH2.
+    * eapply mem_unchanged_on_sub; [ eassumption | intros; simpl ].
+      unfold vis in *; simpl in *; trivial.
+    * intros. exploit UNCH3; clear UNCH3.
+      ++ eapply mem_unchanged_on_sub; [ eassumption | intros; simpl ].
+         unfold vis in *; simpl in *. red; intros. ; trivial.
+         red; intros.
+Search Mem.unchanged_on.
+
+  - admit. - admit.
+  - admit. (* destruct A1; destruct A2; destruct A3; simpl in *; try contradiction.
+    * rename c into c1'. rename m into m1'. rename m0 into m2'. 
+      rename c4 into c3'. rename m4 into m3'. 
+      red in LOCALLOC12. red in LOCALLOC23.
+      destruct mu12; destruct mu12'; simpl in *.
+      destruct REL12 as [INJ12' [E12 [MRR1 [MRR2 [VINJ12 X12]]]]].
+      destruct REL23 as [INJ23' [E23 [MRR2' [MRR3 [VINJ23 X23]]]]]. red.*)
+  - admit. (* clear - REL12 REL23. destruct A1; destruct A2; destruct A3; simpl in *; try contradiction.
+    * rename c into c1'. rename m into m1'. rename m0 into m2'. 
+      rename c4 into c3'. rename m4 into m3'. *)
+  - clear - UNCH3 H H1.
+
+econstructor.
+
+
+Definition WP_trans:
+        Wholeprog_sim.Wholeprog_sim Sem1 Sem3 g1 g3 Main GeInv13 (InitInv13 g2) (HaltInv13 g2).
+
 
   (** The clause that relates initial states. *)
 ; core_initial :
@@ -200,7 +425,8 @@ Record SM_simulation_inject := {
                exists b1 delta1,
                  foreign_of mu b1 = Some(b,delta1)
                  /\ U1 b1 (ofs-delta1) = true
-                 /\ Mem.perm m1 b1 (ofs-delta1) Max Nonempty)))
+                 /\ (*in fact, other properties of effstep already 
+                      imply this conjunct:*) Mem.perm m1 b1 (ofs-delta1) Max Nonempty)))
 
   (** The clause that relates halted states. *)
 ; core_halted :
